Work a little on syntactic proofs

compiler/backend/proofs/clos_callProofScript.sml
@@ -1553,6 +1553,9 @@ val compile_inc_def = Define `
   compile_inc g (e,xs) =
     let (ea, g') = calls [e] g in (g', HD ea, [])`;
 
+val syntax_ok_def = Define`
+  syntax_ok x ⇔ every_Fn_SOME x ∧ every_Fn_vs_NONE x ∧ ALL_DISTINCT (code_locs x)`;
+
 val code_inv_def = Define `
   code_inv (s_code:num |-> num # closLang$exp) s_cc s_co t_code t_cc t_co <=>
     s_code = FEMPTY /\
@@ -3682,8 +3685,7 @@ val semantics_compile = Q.store_thm("semantics_compile",
   `semantics ffi max_app FEMPTY co cc x ≠ Fail ∧
    compile do_call x = (y,aux) ∧
    (if do_call then
-    every_Fn_SOME x ∧ every_Fn_vs_NONE x ∧
-    ALL_DISTINCT (code_locs x) ∧
+    syntax_ok x ∧
     code_inv FEMPTY cc co (FEMPTY |++ aux) cc1 co1
     else cc = state_cc (CURRY I) cc1 ∧
          co1 = state_co (CURRY I) co) ⇒
@@ -3695,7 +3697,7 @@ val semantics_compile = Q.store_thm("semantics_compile",
   \\ fs[FUPDATE_LIST_THM]
   >- ( match_mp_tac semantics_CURRY_I \\ fs[] )
   \\ irule semantics_calls
-  \\ fs[compile_def]);
+  \\ fs[compile_def, syntax_ok_def]);
 
 (* Preservation of some label properties
   every_Fn_SOME xs ∧ every_Fn_vs_NONE xs
